theorem about elections once 0s are removed

src/sf_proof.v
@@ -34,13 +34,15 @@ Ltac unfold_defs := cbv [sf_imp.no_viable_candidates sf_spec.no_viable_candidate
                          sf_imp.eliminated sf_imp.no_viable_candidates_selection
                         in_record sf_spec.overvote sf_spec.properly_selects
                         sf_spec.does_not_select eq_dec sf_spec.selected_candidate
-                        sf_spec.continuing_ballot sf_spec.exhausted_ballot].
+                        sf_spec.continuing_ballot sf_spec.exhausted_ballot
+                        sf_spec.selected_candidate].
 
 Ltac unfold_defs_star := cbv [sf_imp.no_viable_candidates sf_spec.no_viable_candidates
                          sf_imp.eliminated sf_imp.no_viable_candidates_selection in_record 
                          sf_spec.overvote sf_spec.properly_selects
                          sf_spec.does_not_select eq_dec sf_spec.selected_candidate
-                         sf_spec.continuing_ballot sf_spec.exhausted_ballot] in *.
+                         sf_spec.continuing_ballot sf_spec.exhausted_ballot
+                         sf_spec.selected_candidate] in *.
 
 
 Tactic Notation "unfold_defs" "in" "*" := unfold_defs_star.
@@ -134,6 +136,7 @@ match goal with
 | [ H : Some _ = Some _ |- _] => inv H
 | [ |- ~_ ] => intro
 | [ H :  sf_spec.next_ranking _ _ [] _ |- _ ] => inv H
+| [ H : exists _, _ |- _ ] => destruct H
 end.
 
 Ltac unique :=
@@ -1763,6 +1766,276 @@ in_record ([loser] :: rec).
 intros. extensionality c. apply update_eliminated_in_rec_eq.
 Qed.
 
+Definition continuing2 b rec:=
+exists r, sf_spec.next_ranking candidate rec b r /\ ~sf_spec.overvote candidate r.
+
+
+Lemma continuing2_continuing : 
+forall b rec,
+continuing2 b rec <-> sf_spec.continuing_ballot candidate rec b.
+Proof.
+intros.
+split.
+intros.
+unfold continuing2 in *.
+solve_rcv.
+destruct H1. apply H1. exists x. auto.
+destruct H1. solve_rcv.
+eapply sf_spec.next_ranking_unique in H; eauto. subst.
+apply H0; eauto.
+intros.
+unfold continuing2.
+solve_rcv.
+
+apply Classical_Prop.not_or_and in H.
+destruct H. apply Classical_Prop.NNPP in H.
+destruct H. exists x.
+split. auto.
+intro. apply H0. exists x. auto.
+Qed.
+
+Lemma continuing_ballot_cons :
+forall r h t,
+sf_spec.continuing_ballot candidate r (h :: t) ->
+sf_spec.continuing_ballot candidate r [h] \/ ((~sf_spec.overvote candidate h) /\ sf_spec.continuing_ballot candidate r t).
+Proof.
+intros. repeat rewrite <- continuing2_continuing in *.
+induction t. 
+- auto.
+- unfold continuing2 in *.
+  destruct H. destruct H.
+  inv H.
+  + right. intuition. exists x. auto.
+  + destruct H5. 
+    *  intuition. 
+    * left. exists x.
+      intuition. eapply sf_spec.next_ranking_valid.
+      apply H3. auto.
+Qed.
+
+Lemma continuing_ballot_cons2 :
+forall r a b,
+sf_spec.continuing_ballot candidate r [a] ->
+sf_spec.continuing_ballot candidate r (a :: b).
+Proof.
+intros. rewrite <- continuing2_continuing in *.
+unfold continuing2 in *. destruct H.
+exists x.
+destruct H. intuition.
+clear H0.
+inv H. inv H5. eapply sf_spec.next_ranking_valid; eauto.
+Qed.
+
+Lemma continuing_ballot_cons3 :
+forall t h r
+(OV : ~sf_spec.overvote candidate h), 
+sf_spec.continuing_ballot candidate r t ->
+sf_spec.continuing_ballot candidate r (h :: t).
+Proof.
+intros. rewrite <- continuing2_continuing in *.
+unfold continuing2 in *.
+destruct H. destruct H.
+destruct (classic (Forall r h)).
+exists x. intuition. 
+constructor; eauto.
+destruct h. exfalso. solve_rcv. apply H1. solve_rcv.
+exists (c::h). intuition.
+eapply sf_spec.next_ranking_valid. simpl. eauto. 
+right. solve_rcv. apply H1. intros. destruct H3. subst. auto.
+destruct (rel_dec_p c x0).
+subst. auto.
+exfalso. apply OV. exists c. exists x0.
+simpl. auto.
+Qed.
+
+Lemma continuing_ballot_rec_cons : 
+forall l r b,
+  sf_spec.continuing_ballot candidate (in_record ([l] :: r)) (b) ->
+   sf_spec.continuing_ballot candidate (in_record r) (b).
+Proof.
+  intros. induction b.
+  - unfold sf_spec.continuing_ballot in *.  
+    intro. apply H. clear H.
+    unfold sf_spec.exhausted_ballot. left. intro.
+    inv H. inv H1.
+  - apply continuing_ballot_cons in H.  
+    destruct H.
+    apply continuing_ballot_cons2. 
+    rewrite <- continuing2_continuing in *.
+    unfold continuing2. 
+    unfold continuing2 in H.
+    destruct H. exists x.
+    destruct H. intuition.
+    inv H. constructor; solve_rcv.
+    destruct H5. intuition.
+    eapply sf_spec.next_ranking_valid; eauto.
+    right. intro. apply H; clear H.
+    unfold in_record in *. solve_rcv.
+    intuition.
+    apply continuing_ballot_cons3; auto.
+Qed.
+
+Lemma next_ranking_cons_or2 :
+forall b1 bal e x,
+sf_spec.next_ranking candidate e (b1 :: bal) x ->
+sf_spec.next_ranking candidate e [b1] x \/ 
+(Forall e b1 /\ sf_spec.next_ranking candidate e bal x).
+intros. inv H; solve_rcv. left.
+destruct H4; solve_rcv. eapply sf_spec.next_ranking_valid; solve_rcv.
+left. eauto. eapply sf_spec.next_ranking_valid; solve_rcv.
+Qed.
+
+Lemma continuing_ballot_cons4 : (*should be main lemma, don't want to rework proofs :( *)
+forall r h t,
+sf_spec.continuing_ballot candidate r (h :: t) ->
+sf_spec.continuing_ballot candidate r [h] \/ ((~sf_spec.overvote candidate h) /\ sf_spec.continuing_ballot candidate r t /\ Forall r h).
+Proof.
+intros. repeat rewrite <- continuing2_continuing in *.
+induction t. 
+- auto.
+- unfold continuing2 in *.
+  destruct H. destruct H.
+  inv H.
+  + right. intuition. exists x. auto.
+  + destruct H5. 
+    *  intuition. 
+    * left. exists x.
+      intuition. eapply sf_spec.next_ranking_valid.
+      apply H3. auto.
+Qed.
+
+Lemma selected_cons :
+forall r a b c,
+sf_spec.selected_candidate candidate  r (a :: b) c ->
+sf_spec.selected_candidate candidate r [a] c \/
+(Forall r a /\ ~sf_spec.overvote candidate a /\sf_spec.selected_candidate candidate r b c).
+Proof.
+intros.
+unfold sf_spec.selected_candidate in H.
+intuition_nosplit. apply continuing_ballot_cons4 in H.
+apply next_ranking_cons_or2 in H0.
+destruct H, H0.
+left. unfold sf_spec.selected_candidate. intuition.
+eauto.
+rewrite <- continuing2_continuing in H.
+unfold continuing2 in H. destruct H. destruct H.
+inv H. inv H8. rewrite Forall_forall in H0. intuition.
+destruct H. destruct H2. inv H0. inv H9. rewrite Forall_forall in *.
+intuition.
+right. unfold sf_spec.selected_candidate. intuition.
+eauto.
+Qed.
+
+Lemma first_choices_0_cons :
+forall r c h t,
+sf_spec.first_choices candidate r c (h :: t) 0 <->
+sf_spec.first_choices candidate r c [h] 0 /\
+sf_spec.first_choices candidate r c t 0.
+Proof.
+split.
+- intros.
+  induction t. intuition. constructor.
+  inv H. intuition.
+  inv H4.
+  apply IHt.
+  constructor. auto. auto.
+- intros. destruct H.
+  inv H. constructor; auto.
+Qed.
+
+Lemma next_ranking_record_same :
+forall b x c l r,
+  In c x ->
+  c <> l ->
+  sf_spec.next_ranking candidate (in_record r) b x ->
+  ~ sf_spec.overvote candidate x ->
+  sf_spec.next_ranking candidate (in_record ([l] :: r)) b x.
+Proof.
+induction b; intros.
+inv H1.
+inv H1.
+- constructor. solve_rcv. specialize (H5 x0); solve_rcv.
+  auto.
+  eapply IHb; eauto.
+- intuition.
+  eapply sf_spec.next_ranking_valid.
+  apply H5. right. intro.
+  apply H1. solve_rcv. simpl in H3. destruct H3; solve_rcv.
+  assert (c0 = l). inv H4. subst; intuition. inv H3. subst. clear H4.
+  exfalso. apply H2. exists c. exists l. eauto.
+Qed.
+
+Lemma ne_still_continuing :
+forall b c l  x r,
+sf_spec.next_ranking candidate (in_record r) b x ->
+sf_spec.continuing_ballot candidate (in_record r) b ->
+In c x ->
+c <> l ->
+sf_spec.continuing_ballot candidate (in_record ([l] :: r)) b.
+Proof.
+intros. repeat rewrite <- continuing2_continuing in *.
+unfold continuing2 in *. intuition_nosplit.
+exists x0. split; eauto. 
+eapply sf_spec.next_ranking_unique in H; eauto. subst.
+eapply next_ranking_record_same; eauto.
+Qed.
+
+Lemma selected_rec_cons :
+forall r b c l,
+c <> l ->
+sf_spec.selected_candidate candidate (in_record r) b c ->
+sf_spec.selected_candidate candidate (in_record ([l]::r)) b c.
+intros.
+induction b. solve_rcv.
+apply selected_cons in H0. 
+destruct H0. 
+- clear IHb. 
+  unfold sf_spec.selected_candidate in *.
+  intuition_nosplit.
+  split. 
+  + apply continuing_ballot_cons2. 
+  eapply ne_still_continuing; eauto.
+  + inv H1. inv H8.
+    destruct H7. exists x. intuition.
+    eapply sf_spec.next_ranking_valid; eauto.
+    exists x. intuition. eapply sf_spec.next_ranking_valid; eauto.
+    right. intro. apply H1. rewrite <- continuing2_continuing in *. 
+    unfold continuing2 in *. unfold in_record in *. intuition_nosplit. 
+    simpl in *. destruct H3; subst; try solve [solve_rcv].
+    inv H4; intuition_nosplit. inv H0. inv H10. intuition.
+    exfalso. apply H6. solve_rcv.
+- intuition. clear H3. 
+  unfold sf_spec.selected_candidate in *.
+  intuition_nosplit. split. 
+  rewrite <- continuing2_continuing. unfold continuing2. exists x.
+  intuition. constructor; auto. rewrite Forall_forall in *.
+  intro. specialize (H1 x0). intro. intuition. 
+  solve_rcv.  rewrite <-  continuing2_continuing in *.
+  unfold continuing2 in *. intuition_nosplit.
+  eapply sf_spec.next_ranking_unique in H2; eauto. subst.
+  auto.
+  exists x. intuition.
+  constructor; auto.
+  rewrite Forall_forall in *. intros. specialize (H1 x0). 
+  solve_rcv.
+Qed.
+
+Lemma first_choices_rec_0 :
+forall c l r e,
+  sf_spec.first_choices candidate (in_record ([l] :: r)) c e 0 ->
+  c <> l ->
+  sf_spec.first_choices candidate (in_record r) c e 0.
+Proof.
+intros.
+induction e.
+- constructor.
+- apply first_choices_0_cons in H. destruct H. intuition.
+  apply first_choices_0_cons. intuition.
+  inv H.
+  constructor. intro. apply H5. clear H5. 
+  apply selected_rec_cons; auto. constructor.
+Qed.
+
 Lemma run_election'_correct : 
   forall fuel election winner rec' rec tbreak
          (TB : forall c x, tbreak c = Some x -> In x c) 
@@ -1791,7 +2064,7 @@ induction fuel; intros.
       eapply total_selected_unique; eauto. }
     subst. 
     rewrite sf_imp.gtb_nat_gt in Heqb. auto. apply _.
-  + unfold sf_imp.find_eliminated_noopt in *.
+  + unfold sf_imp.find_eliminated_noopt in *. 
     destruct (tbreak (sf_imp.get_bottom_votes candidate l)) eqn:?. 
     * rename c0 into loser.
       rename Heqo0 into TBREAK.
@@ -1849,18 +2122,20 @@ induction fuel; intros.
               destruct H0.
               exists x. intuition.
               clear - H1 n0.
-             
+              eapply first_choices_rec_0; eauto.
+          + 
 
-Lemma first_choices_rec_0 :
-forall c l r e,
-  sf_spec.first_choices candidate (in_record ([l] :: r)) c e 0 ->
-  c <> l ->
-  sf_spec.first_choices candidate (in_record r) c e 0.
-Proof.
-intros.
-inv H. 
-- constructor.
-- constructor. intro. apply H1.
+
+Lemma next_ranking_rec_ne :
+forall b r c l x,
+ c <> l ->
+ sf_spec.continuing_ballot candidate (in_record r) b ->
+ sf_spec.next_ranking candidate (in_record r) b x ->
+ In c x ->
+ sf_spec.next_ranking candidate (in_record ([l] :: r)) b x.
+proo
+
+
 
 Lemma next_ranking_no_viable : forall a l r  x,
 sf_spec.next_ranking _ (in_record r) a x ->
@@ -1961,7 +2236,7 @@ sf_spec.next_ranking candidate (in_record r) a x ->
 ~sf_spec.overvote candidate (in_record r) a ->
 sf_spec.overvote candidate (in_record ([l] :: r)) a ->
 Forall (eq l) x.
-induction a; intros.
+  induction a; intros.
 - simpl in *. inv H.
 - simpl in H. destruct H.
   + destruct H. apply eliminated_overvote_cons in H1; auto.
